Updated Hoare logic with an extensible record

HL_State.thy
@@ -1,16 +1,10 @@
-theory State_Monad_HL
+theory HL_State
 imports 
   Main
   "~~/src/HOL/Library/State_Monad"
 begin
 
 section\<open>Introduction\<close>
-text\<open>This report presents the proof of the Dutch National Flag Problem in Isabelle using a Hoare Calculus defined by Stefan Hallerstede. 
-    The proof has been carried out using this calculus by Simon Thrane Hansen as a part of some learning exercises. 
-    This document serves as a technical report of the proof and presents the Hoare calculus. The document first presents the Hoare calculus. 
-    Afterward comes a presentation of the algorithm and its properties. After this, follows all the definitions of both the method-definitions and their corresponding pre- and post-conditions. 
-    This section gets followed by the proofs of the definitions. Finally, the algorithm is defined as a recursive function which gets proved in the final part of the report.\<close>
-
 
 section\<open>Hoare calculus\<close>
 text\<open>Basic definitions that can be useful inside as a parameter to spec in a proof\<close>
@@ -24,8 +18,68 @@ text\<open>Methods to get describe the basic state changes. These are described 
 definition return:: "'a \<Rightarrow> ('b, 'a) state" where "return = State_Monad.return"
 definition get_state:: "('a, 'a) state" where "get_state = State (\<lambda>x. (x,x))"
 definition put_state:: "'a \<Rightarrow> ('a, unit) state" where "put_state x = State (\<lambda>_. ((),x))"
-definition skip:: "('a, unit) state" where "skip = State (\<lambda>x. ((),x))"
 
+definition unpack_state:: "('a, unit) state \<Rightarrow> 'a \<Rightarrow> 'a" where 
+  "unpack_state S x \<equiv> snd(run_state S x)"
+
+
+type_synonym 'a bexp = "'a \<Rightarrow> bool"
+type_synonym 'a assn = "'a \<Rightarrow> bool"
+
+subsubsection\<open>Commands\<close>
+text\<open>Commands describe that can be done in the langagauge.\<close>
+text\<open>I have assumed that all calls eventually be reduces to basic commands which involves manipulation of the state-monad.\<close>
+datatype 'a com =
+  Basic "('a, unit) state"
+| Seq  "'a com" "'a com"                     ("(_;/ _)"      [61,60] 60)
+| Cond "'a bexp" "'a com" "'a com"           ("(1IF _/ THEN _ / ELSE _/ FI)"  [0,0,0] 61)
+
+text\<open>The skip-command is just a special command which leaves the state-monad unchanged. Put monad-identify - this should be a return\<close>
+abbreviation annskip ("SKIP") where "SKIP == (State_Monad.return)"
+
+type_synonym 'a sem = "('a, unit) state  => ('a, unit) state => bool"
+
+text\<open>This could potentially be useful in the while-loop. 
+  It states that the predicate is not longer true in the base case, but that the final state has also been reached.
+  The other case states that be predicate is true and it is possible to reach the base-case in a finite amount of steps.
+ It is taken from: \url{http://isabelle.in.tum.de/dist/library/HOL/HOL-Isar_Examples/Hoare.html}\<close>
+(*primrec iter :: "nat \<Rightarrow> 'a bexp \<Rightarrow> 'a sem \<Rightarrow> 'a sem"
+  where
+    "iter 0 b S s s' \<longleftrightarrow> \<not>b s \<and> s = s'"
+  | "iter (Suc n) b S s s' \<longleftrightarrow> b s \<and> (\<exists>s''. S s s'' \<and> iter n b S s'' s')"
+*)
+
+text\<open>The semantics describe how the program should be interpreted. It takes a command and returns two states - the pre and post state of each command.\<close>
+inductive Sem :: "'a com \<Rightarrow> 'a sem"
+where
+  "Sem (Basic f) s (f)"
+| "Sem c1 s s'' \<Longrightarrow> Sem c2  s'' s' \<Longrightarrow> Sem (c1;c2) s s'"
+| "b s \<Longrightarrow> Sem c1 s s' \<Longrightarrow> Sem (IF b THEN c1 ELSE c2 FI) s s'"
+| "\<not>b s \<Longrightarrow> Sem c2 s s' \<Longrightarrow> Sem (IF b THEN c1 ELSE c2 FI) s s'"
+
+inductive_cases [elim!]:
+  "Sem (Basic f) s s'" 
+  "Sem (c1;c2) s s'"
+  "Sem (IF b THEN c1 ELSE c2 FI) s s'"
+
+definition Valid :: "'a bexp \<Rightarrow> 'a com \<Rightarrow> 'a bexp \<Rightarrow> bool"
+  where "Valid p c q \<longleftrightarrow> (\<forall>s s'. Sem c s s' \<longrightarrow>  p s \<longrightarrow> q (unpack_state s' s))"
+
+lemma SkipRule: "p = q \<Longrightarrow> Valid p SKIP q"
+by (auto simp:Valid_def)
+
+lemma BasicRule: "\<forall>s. p s \<longrightarrow> q (unpack_state (f s) s) \<Longrightarrow> Valid p (Basic f) q"
+  by (auto simp:Valid_def)
+
+lemma SeqRule: "Valid p c1 q  \<Longrightarrow> Valid q c2 r  \<Longrightarrow> Valid p (c1;c2) r"
+  apply (auto simp:Valid_def)
+  sorry
+
+
+lemma CondRule:
+ "\<forall>s. p s \<longrightarrow> ((b s \<longrightarrow> w s) \<and> (\<not>b s \<longrightarrow>  w' s))
+  \<Longrightarrow> Valid w c1 q \<Longrightarrow> Valid w' c2 q \<Longrightarrow> Valid p (Cond b c1 c2) q"
+  by (auto simp:Valid_def)
 
 definition get:: "('a \<Rightarrow> 'b) \<Rightarrow> ('a, 'b) state" where 
   "get v = do { x \<leftarrow> get_state; return (v x) }"
@@ -34,7 +88,19 @@ definition put:: "('a \<Rightarrow> 'b \<Rightarrow> 'a) \<Rightarrow> 'b \<Righ
   "put vu a = do { x \<leftarrow> get_state; put_state (vu x a) }"
 
 definition assign:: "('a \<Rightarrow> 'b \<Rightarrow> 'a) \<Rightarrow> ('a \<Rightarrow> 'b) \<Rightarrow> ('a, unit) state" where
-  "assign vu v = do { a \<leftarrow> get v; put vu a }"
+  "assign vu v =  (do { a \<leftarrow> get v; put vu a })"
+
+definition assign1 :: "('a \<Rightarrow> 'b \<Rightarrow> 'a) \<Rightarrow> ('a \<Rightarrow> 'b) \<Rightarrow> 'a com" ("(2_ :=/ _)" [70, 65] 61) where 
+  "assign1 vu v = Basic (\<lambda>e. do { a \<leftarrow> get v; put vu a })" 
+
+text\<open>This is what enables the \<close>
+syntax
+  "_hoare_vars" :: "[idts, 'a assn,'a com,'a assn] \<Rightarrow> bool" ("(VARS _ //{_} // _ // {_})" [0,0,55,0] 50)
+
+text\<open>This is what enables the \<close>
+syntax
+  "_hoare" :: "['a assn,'a com,'a assn] => bool" ("({_} // _ // {_})" [0,55,0] 50)
+
 
 definition spec:: "('a \<Rightarrow> bool) \<Rightarrow> ('a, 'b) state \<Rightarrow> ('b \<Rightarrow> 'a \<Rightarrow> bool) \<Rightarrow> bool" where 
   "spec p S q = (\<forall>x. p x  \<longrightarrow> (let (y, z) = run_state S x in q y z))"
@@ -43,6 +109,7 @@ subsection\<open>Hoare logic\<close>
 text\<open>Rules based on section 3 in Verification of Sequential and Concurrent Programs\<close>
 theorem get_state_rule: "spec (\<lambda>x. p x x) (get_state) p"
   by (simp add: get_state_def spec_def)
+
 
 text\<open>Rule to extract a value from the Monad\<close>
 theorem get_rule: "\<forall>x. spec (\<lambda>y. p y \<and> v x = v y) (S (v x)) q \<Longrightarrow> spec p (get v \<bind> S) q"
@@ -61,9 +128,6 @@ text\<open>Rule to capture scope of local variables\<close>
 theorem let_rule: "let v = E in spec p (do { T }) r \<Longrightarrow> spec p (do { let v = E; T }) r"
   by (simp add: spec_def snd_def)
 
-text\<open>A skip-statement can be ignored\<close>
-theorem skip_left_rule: "spec p (do { skip; S }) q \<Longrightarrow> spec p S q"
-  by (simp add: spec_def skip_def)
 
 text\<open>Pre- and post-conditions can be conjoined\<close>
 theorem conj_rule: "\<lbrakk>spec p S q; spec r S s\<rbrakk> \<Longrightarrow> spec (\<lambda>x. p x \<and> r x) S (\<lambda>x y. q x y \<and> s x y)"
@@ -87,5 +151,6 @@ theorem strengthen_rule: "\<lbrakk>\<forall>x y. (q0 x y \<longrightarrow> q x y
 text\<open>A conditional statement can be split up into multiple proofs with difference assumptions (based on the queteria)\<close>
 theorem cond_rule: "\<lbrakk>spec (\<lambda>x. p x \<and> b) S q; spec (\<lambda>x. p x \<and> \<not>b) T q\<rbrakk> \<Longrightarrow> spec p (if b then S else T) q"
   by (simp add: spec_def)
+
 
 end
