State_Monad_HL.thy
@@ -10,20 +10,25 @@ definition FF:: "'a \<Rightarrow> bool" where "FF x = False"
 definition GG:: "('a \<Rightarrow> bool) \<Rightarrow> ('b => 'a \<Rightarrow> bool)" where "GG p x = p"
 definition UU:: "('a \<Rightarrow> bool) \<Rightarrow> (unit => 'a \<Rightarrow> bool)" where "UU p x = p"
 
-definition return:: "'a \<Rightarrow> ('b, 'a) state" where "return = State_Monad.return"
-definition get_state:: "('a, 'a) state" where "get_state = State (\<lambda>x. (x,x))"
-definition put_state:: "'a \<Rightarrow> ('a, unit) state" where "put_state x = State (\<lambda>_. ((),x))"
-definition skip:: "('a, unit) state" where "skip = State (\<lambda>x. ((),x))"
+                  
+record status =
+    ok:: bool
 
-definition get:: "('a \<Rightarrow> 'b) \<Rightarrow> ('a, 'b) state" where 
+definition return:: "'a \<Rightarrow> (status + 'b, 'a) state" where "return = State_Monad.return"
+definition get_state:: "(status + 'a, status + 'a) state" where "get_state = State (\<lambda>x. (x,x))"
+definition put_state:: "status + 'a \<Rightarrow> (status + 'a, unit) state" where "put_state x = State (\<lambda>_. ((),x))"
+definition skip:: "(status + 'a, unit) state" where "skip = State (\<lambda>x. ((),x))"
+
+definition get:: "(status + 'a \<Rightarrow> 'b) \<Rightarrow> (status + 'a, 'b) state" where 
   "get v = do { x \<leftarrow> get_state; return (v x) }"
-definition put:: "('a \<Rightarrow> 'b \<Rightarrow> 'a) \<Rightarrow> 'b \<Rightarrow> ('a, unit) state" where 
+
+definition put:: "(status + 'a \<Rightarrow> 'b \<Rightarrow> status + 'a) \<Rightarrow>  'b \<Rightarrow> (status + 'a, unit) state" where 
   "put vu a = do { x \<leftarrow> get_state; put_state (vu x a) }"
 
-definition assign:: "('a \<Rightarrow> 'b \<Rightarrow> 'a) \<Rightarrow> ('a \<Rightarrow> 'b) \<Rightarrow> ('a, unit) state" where
+definition assign:: "(status + 'a \<Rightarrow> 'b \<Rightarrow> status + 'a) \<Rightarrow> (status + 'a \<Rightarrow> 'b) \<Rightarrow> (status + 'a, unit) state" ("(2_ :=/ _)" [70, 65] 61) where
   "assign vu v = do { a \<leftarrow> get v; put vu a }"
 
-definition spec:: "('a \<Rightarrow> bool) \<Rightarrow> ('a, 'b) state \<Rightarrow> ('b \<Rightarrow> 'a \<Rightarrow> bool) \<Rightarrow> bool" where 
+definition spec:: "(status + 'a \<Rightarrow> bool) \<Rightarrow> (status +  'a, 'b) state \<Rightarrow> ('b \<Rightarrow> status +  'a \<Rightarrow> bool) \<Rightarrow> bool" where 
   "spec p S q = (\<forall>x. p x  \<longrightarrow> (let (y, z) = run_state S x in q y z))"
 
 theorem get_state_rule: "spec (\<lambda>x. p x x) (get_state) p"
@@ -34,6 +39,11 @@ theorem get_rule: "\<forall>x. spec (\<lambda>y. p y \<and> v x = v y) (S (v x))
 
 theorem return_rule: "spec (p v) (return v) p"
   by (simp add: return_def spec_def)
+
+(*
+theorem assign_rule: "spec (p) (assign vu v) p"
+  by (simp add: return_def spec_def)
+*)
 
 theorem seq_rule: "\<lbrakk>spec p S q; \<forall>x. spec (q x) T r\<rbrakk> \<Longrightarrow> spec p (do { S; T }) r"
   apply (simp add: spec_def)
@@ -62,5 +72,7 @@ theorem strengthen_rule: "\<lbrakk>\<forall>x y. (q0 x y \<longrightarrow> q x y
 
 theorem cond_rule: "\<lbrakk>spec (\<lambda>x. p x \<and> b) S q; spec (\<lambda>x. p x \<and> \<not>b) T q\<rbrakk> \<Longrightarrow> spec p (if b then S else T) q"
   by (simp add: spec_def)
+
+(*While loop and extensive records of state. Read chapters 0-4.*)
 
 end
